```markdown
import Mathlib.Analysis.Calculus.Deriv
import Mathlib.Analysis.SpecialFunctions.Trigonometric
import Mathlib.Analysis.SpecialFunctions.Hyperbolic
import Mathlib.Data.Set.Basic
import Mathlib.Topology.Basic
import Mathlib.Topology.ContinuousFunction.Basic

open Real
open Set

def putnam_1963_b3_solution : Set (ℝ → ℝ) :=
  {f | ∃ (A : ℝ) (k : ℝ), ∀ u : ℝ, f u = A * Real.sinh (k * u)} ∪
  {f | ∃ (A : ℝ), ∀ u : ℝ, f u = A * u} ∪
  {f | ∃ (A : ℝ) (k : ℝ), ∀ u : ℝ, f u = A * Real.sin (k * u)}

theorem putnam_1963_b3
    (f : ℝ → ℝ) :
    f ∈ putnam_1963_b3_solution ↔
      (ContDiff ℝ 2 f ∧
      ∀ x y : ℝ, (f x) ^ 2 - (f y) ^ 2 = f (x + y) * f (x - y)) :=
  by
  constructor
  -- (⇒)
  · intro hf
    constructor
    · -- ContDiff ℝ 2 f
      cases hf
      case inl hAksinh =>
        rcases hAksinh with ⟨A, k, hf⟩
        have hf' : f = fun u => A * Real.sinh (k * u) := by ext u; exact hf u
        rw [hf']
        exact ContDiff.const_mul (ContDiff.sinh (ContDiff.const_mul contDiff_id (ContDiff.const k)))

      case inr hrest =>
        cases hrest
        case inl hAu =>
          rcases hAu with ⟨A, hf⟩
          have hf' : f = fun u => A * u := by ext u; exact hf u
          rw [hf']
          exact ContDiff.const_mul contDiff_id (ContDiff.const A)
        case inr hAksin =>
          rcases hAksin with ⟨A, k, hf⟩
          have hf' : f = fun u => A * Real.sin (k * u) := by ext u; exact hf u
          rw [hf']
          exact ContDiff.const_mul (ContDiff.sin (ContDiff.const_mul contDiff_id (ContDiff.const k)))
    · -- ∀ x y : ℝ, (f x) ^ 2 - (f y) ^ 2 = f (x + y) * f (x - y)
      intro x y
      cases hf
      case inl hAksinh =>
        rcases hAksinh with ⟨A, k, hf⟩
        simp [hf x, hf y, hf (x+y), hf (x-y), Real.sinh]
        have : (A * Real.sinh (k * x)) ^ 2 - (A * Real.sinh (k * y)) ^ 2 = A^2 * (Real.sinh (k * x) ^ 2 - Real.sinh (k * y) ^ 2) := by ring
        rw [this]
        have : (A * Real.sinh (k * (x + y))) * (A * Real.sinh (k * (x - y))) = A^2 * (Real.sinh (k * (x + y)) * Real.sinh (k * (x - y))) := by ring
        rw [this]
        have : Real.sinh (k * (x + y)) * Real.sinh (k * (x - y)) = Real.sinh (k * x + k * y) * Real.sinh (k * x - k * y) := by ring
        rw [this]
        rw [Real.sinh_add]
        rw [Real.sinh_sub]
        ring
      case inr hrest =>
        cases hrest
        case inl hAu =>
          rcases hAu with ⟨A, hf⟩
          simp [hf x, hf y, hf (x+y), hf (x-y)]
          ring
        case inr hAksin =>
          rcases hAksin with ⟨A, k, hf⟩
          simp [hf x, hf y, hf (x+y), hf (x-y)]
          have : (A * Real.sin (k * x)) ^ 2 - (A * Real.sin (k * y)) ^ 2 = A^2 * (Real.sin (k * x) ^ 2 - Real.sin (k * y) ^ 2) := by ring
          rw [this]
          have : (A * Real.sin (k * (x + y))) * (A * Real.sin (k * (x - y))) = A^2 * (Real.sin (k * (x + y)) * Real.sin (k * (x - y))) := by ring
          rw [this]
          have : Real.sin (k * (x + y)) * Real.sin (k * (x - y)) = Real.sin (k * x + k * y) * Real.sin (k * x - k * y) := by ring
          rw [this]
          rw [Real.sin_add]
          rw [Real.sin_sub]
          ring
  -- (⇐)
  · intro h
    have hcd : ContDiff ℝ 2 f := h.1
    have hfe : ∀ x y : ℝ, (f x) ^ 2 - (f y) ^ 2 = f (x + y) * f (x - y) := h.2

    --substituting y = 0
    have hfe_y0 : ∀ x : ℝ, (f x) ^ 2 - (f 0) ^ 2 = f (x) * f (x) := by
      intro x
      specialize hfe x 0
      simp [hfe]

    --claim f(0) = 0 or f(x) = 0
    have hclaim : f 0 = 0 ∨ (∀ x : ℝ, f x = 0) := by
      by_cases hf0 : f 0 = 0
      · left
        exact hf0
      · right
        intro x
        have hx : (f x)^2 - (f 0)^2 = f x * f x := hfe_y0 x
        have : f 0 ≠ 0 := hf0
        have : (f x)^2 - (f 0)^2 = (f x)^2 := by simp [pow_two, mul_eq_zero]
        rw [this] at hx
        have : (f x)^2 = (f x)^2 := by simp
        rw [this] at hx
        simp at hx
        exact hx
    --cases f(0) = 0
    cases hclaim
    case inl hf0 =>
      have hfe_y0' : ∀ x : ℝ, (f x) ^ 2 = f (x) * f (x) := by
        intro x
        specialize hfe_y0 x
        simp [hf0] at hfe_y0
        exact hfe_y0
      have hfe_0y : ∀ y : ℝ, (f 0) ^ 2 - (f y) ^ 2 = f (0 + y) * f (0 - y) := by
        intro y
        specialize hfe 0 y
        exact hfe
      have hfe_0y' : ∀ y : ℝ, -(f y) ^ 2 = f (y) * f (-y) := by
        intro y
        specialize hfe_0y y
        simp [hf0] at hfe_0y
        exact hfe_0y

      have hfe_x0 : ∀ x : ℝ, (f x) ^ 2 - (f 0) ^ 2 = f (x + 0) * f (x - 0) := by
        intro x
        specialize hfe x 0
        exact hfe
      have hfe_x0' : ∀ x : ℝ, (f x) ^ 2 = (f x)^2 := by
        intro x
        specialize hfe_x0 x
        simp [hf0] at hfe_x0
        exact hfe_x0
      -- Differentiation wrt x
      have hderiv : ∀ x y : ℝ, 2 * f x * deriv f x = deriv f (x+y) * f (x-y) + f (x+y) * deriv f (x-y) := by
        intro x y
        let g : ℝ → ℝ := fun x => (f x) ^ 2 - (f y) ^ 2
        let h : ℝ → ℝ := fun x => f (x + y) * f (x - y)
        have hg' : deriv g x = 2 * f x * deriv f x := by
          have h1 : DifferentiableAt ℝ g x := by
            apply DifferentiableAt.sub
            · apply DifferentiableAt.pow
              · exact (hcd.differentiable ℝ).differentiableAt
              · norm_num
            · apply DifferentiableAt.const
          exact deriv_pow' (f x) 2 (hcd.differentiable ℝ).differentiableAt
        have hh' : deriv h x = deriv f (x+y) * f (x-y) + f (x+y) * deriv f (x-y) := by
          have h1 : DifferentiableAt ℝ h x := by
            apply DifferentiableAt.mul
            · apply DifferentiableAt.comp
              · exact (hcd.differentiable ℝ).differentiableAt
              · apply DifferentiableAt.add (DifferentiableAt.const y) (DifferentiableAt.id x)
            · apply DifferentiableAt.comp
              · exact (hcd.differentiable ℝ).differentiableAt
              · apply DifferentiableAt.sub (DifferentiableAt.id x) (DifferentiableAt.const y)
          apply deriv_mul' (f (x+y)) (f (x-y)) ((hcd.differentiable ℝ).differentiableAt.comp (DifferentiableAt.add (DifferentiableAt.id x) (DifferentiableAt.const y))) ((hcd.differentiable ℝ).differentiableAt.comp (DifferentiableAt.sub (DifferentiableAt.id x) (DifferentiableAt.const y)))
        specialize hfe x y
        have hdiff : deriv g x = deriv h x := by
          apply deriv_congr
          · ext z
            exact hfe
        rw [hg', hh'] at hdiff
        exact hdiff

      --substitute x = 0
      have hderiv_x0 : ∀ y : ℝ, 2 * f 0 * deriv f 0 = deriv f (0+y) * f (0-y) + f (0+y) * deriv f (0-y) := by
        intro y
        specialize hderiv 0 y
        exact hderiv
      have hderiv_x0' : ∀ y : ℝ, 0 = deriv f (y) * f (-y) + f (y) * deriv f (-y) := by
        intro y
        specialize hderiv_x0 y
        simp [hf0] at hderiv_x0
        exact hderiv_x0

      -- f(x) = A*x or f(x) = A*sin(k*x) or f(x) = A*sinh(k*x)
      sorry -- This is where the hard part of the proof would go.
    case inr hfx0 =>
      -- f(x) = 0
      left
      use 0
      use 0
      intro u
      simp

```